Crash safe log example (IV)

examples/log/DiskLogSystemInv.dfy
@@ -28,36 +28,146 @@ module DiskLogSystemInv {
     0 <= idx.idx < LengthFromSuperblock(k, s)
   }
 
+  predicate IsALogSectorBlock(blocks: map<M.LBAType.LBA, M.Sector>, idx: Index)
+  {
+    && var lba := M.LBAType.indexToLBA(idx);
+    && lba in blocks
+    && blocks[lba].LogSector?
+  }
+
   predicate DiskIsValidLog(k: D.Constants, s: M.DiskVariables)
   {
     && DiskHasValidSuperblock(k, s)
     && 0 <= LengthFromSuperblock(k, s)
-    && (forall idx :: IndexValidForDiskLog(k, s, idx) ==> (
-      && var lba := M.LBAType.indexToLBA(idx);
-      && lba in s.blocks
-      && s.blocks[lba].LogSector?
-    ))
+    && (forall idx :: IndexValidForDiskLog(k, s, idx) ==> IsALogSectorBlock(s.blocks, idx))
   }
 
   function ElementFromDiskLog(k: D.Constants, s: M.DiskVariables, idx: Index) : M.L.Element
     requires DiskIsValidLog(k, s)
-    requires 0 <= idx.idx < LengthFromSuperblock(k, s)
+    requires IsALogSectorBlock(s.blocks, idx)
   {
     s.blocks[M.LBAType.indexToLBA(idx)].element
+  }
+
+  predicate StagedTrailsLogLength(k: Constants, s: Variables)
+  {
+    s.machine.stagedLength <= |s.machine.log|
   }
 
   predicate MemoryMatchesDisk(k: Constants, s: Variables)
     requires DiskIsValidLog(k.disk, s.disk)
   {
-    forall idx: Index :: 0 <= idx.idx < |s.machine.log| ==> (
-      && IndexValidForDiskLog(k.disk, s.disk, idx)
+    forall idx: Index :: 0 <= idx.idx < |s.machine.log| && idx.idx < s.machine.stagedLength ==> (
+      && IsALogSectorBlock(s.disk.blocks, idx)
       && s.machine.log[idx.idx] == ElementFromDiskLog(k.disk, s.disk, idx)
     )
+  }
+
+  predicate MachinePersistentWhenReadyMatchesDiskSuperblock(k: Constants, s: Variables)
+    requires DiskHasValidSuperblock(k.disk, s.disk)
+  {
+    s.machine.persistent.Ready? ==> s.machine.persistent.superblock.length == LengthFromSuperblock(k.disk, s.disk) 
   }
 
   predicate Inv(k: Constants, s: Variables)
   {
     && DiskIsValidLog(k.disk, s.disk)
+    && MachinePersistentWhenReadyMatchesDiskSuperblock(k, s)
+    && StagedTrailsLogLength(k, s)
     && MemoryMatchesDisk(k, s)
   }
+
+  lemma InitImpliesInv(k: Constants, s: Variables)
+    requires Init(k, s)
+    ensures Inv(k, s)
+  {
+  }
+
+  lemma NextPreservesMachinePersistentWhenReadyMatchesDiskSuperblock(k: Constants, s: Variables, s': Variables)
+    requires Inv(k, s)
+    requires Next(k, s, s')
+    ensures MachinePersistentWhenReadyMatchesDiskSuperblock(k, s')
+  {
+  }
+
+  lemma NextPreservesDiskIsValidLog(k: Constants, s: Variables, s': Variables)
+    requires Inv(k, s)
+    requires Next(k, s, s')
+    requires MachinePersistentWhenReadyMatchesDiskSuperblock(k, s')
+    ensures DiskIsValidLog(k.disk, s'.disk)
+  {
+    var step :| NextStep(k, s, s', step);
+    match step {
+      case MachineStep(diskOp) => {
+        var step :| M.NextStep(k.machine, s.machine, s'.machine, diskOp, step);
+        match step {
+          case QueryStep(idx: Index, result: M.Element) => { }
+          case FetchSuperblockStep(length: int) => { }
+          case FetchElementStep(idx: Index, element: M.Element) => { }
+          case AppendStep(element: M.Element) => { }
+          case StageElementStep() => {
+            assert forall idx :: IndexValidForDiskLog(k.disk, s.disk, idx) ==> IsALogSectorBlock(s.disk.blocks, idx);
+            assert LengthFromSuperblock(k.disk, s'.disk) == LengthFromSuperblock(k.disk, s.disk);
+            assert forall idx :: IndexValidForDiskLog(k.disk, s.disk, idx) ==> IsALogSectorBlock(s'.disk.blocks, idx);
+            assert forall idx :: IndexValidForDiskLog(k.disk, s'.disk, idx) ==> IsALogSectorBlock(s'.disk.blocks, idx);
+            assert DiskIsValidLog(k.disk, s'.disk);
+          }
+          case FlushStep() => { }
+          case StutterStep() => { }
+        }
+      }
+      case CrashStep => { }
+    }
+  }
+
+  lemma NextPreservesStagedTrailsLogLength(k: Constants, s: Variables, s': Variables)
+    requires Inv(k, s)
+    requires Next(k, s, s')
+    ensures StagedTrailsLogLength(k, s')
+  {
+  }
+
+  lemma NextPreservesMemoryMatchesDisk(k: Constants, s: Variables, s': Variables)
+    requires Inv(k, s)
+    requires Next(k, s, s')
+    requires DiskIsValidLog(k.disk, s'.disk)
+    ensures MemoryMatchesDisk(k, s')
+  {
+    var step :| NextStep(k, s, s', step);
+    match step {
+      case MachineStep(diskOp) => {
+        var step :| M.NextStep(k.machine, s.machine, s'.machine, diskOp, step);
+        match step {
+          case QueryStep(idx: Index, result: M.Element) => { }
+          case FetchSuperblockStep(length: int) => { }
+          case FetchElementStep(idx: Index, element: M.Element) => { }
+          case AppendStep(element: M.Element) => {
+            assert s'.machine.stagedLength == s.machine.stagedLength;
+            assert MemoryMatchesDisk(k, s);
+            assert s'.machine.log == s.machine.log + [element];
+            assert s'.machine.log == s'.machine.log[..|s'.machine.log|-1] + [s'.machine.log[|s'.machine.log|-1]];
+            assert MemoryMatchesDisk(k, s');
+          }
+          case StageElementStep() => { }
+          case FlushStep() => { }
+          case StutterStep() => { }
+        }
+      }
+      case CrashStep => {
+        assert MemoryMatchesDisk(k, s');
+      }
+    }
+  }
+
+  lemma NextPreservesInv(k: Constants, s: Variables, s': Variables)
+    requires Inv(k, s)
+    requires Next(k, s, s')
+    ensures Inv(k, s')
+  {
+    NextPreservesMachinePersistentWhenReadyMatchesDiskSuperblock(k, s, s');
+    NextPreservesDiskIsValidLog(k, s, s');
+    NextPreservesStagedTrailsLogLength(k, s, s');
+    NextPreservesMemoryMatchesDisk(k, s, s');
+  }
 }
+
